theories/Closeout/CB_45.v
@@ -4,711 +4,715 @@ From Coq Require Import List.
 From BBB4 Require Import BBB4_Statement.
 From BBB4.Census Require Import Deferred_Defs.
 From BBB4.Closeout Require Import CloseoutKit.
+Require BBB4.Machines.NGHWStage.NGHW_03.
 Require BBB4.Machines.NGHWStage.NGHW_04.
-Require BBB4.Machines.NGHWStage.NGHW_05.
 Import ListNotations.
 
+(* 1RB1LC_0LC0RB_1LA1RD_1RC0LB *)
+Lemma cov_45_0000 : covers (row_to_tm [t1RB;t1LC;t0LC;t0RB;t1LA;t1RD;t1RC;t0LB]).
+Proof.
+  apply (covers_iqh_at BBB4.Machines.NGHWStage.NGHW_03.tmq_h_00397);
+    [exact BBB4.Machines.NGHWStage.NGHW_03.cqh_h_00397 | intros q s; destruct q, s; reflexivity].
+Qed.
+
+(* 1RB1LC_0LC0RB_1LA1RD_1RC0LD *)
+Lemma cov_45_0001 : covers (row_to_tm [t1RB;t1LC;t0LC;t0RB;t1LA;t1RD;t1RC;t0LD]).
+Proof.
+  apply (covers_iqh_at BBB4.Machines.NGHWStage.NGHW_03.tmq_h_00398);
+    [exact BBB4.Machines.NGHWStage.NGHW_03.cqh_h_00398 | intros q s; destruct q, s; reflexivity].
+Qed.
+
+(* 1RB1LC_0LC0RB_1LA1RD_1RC1LB *)
+Lemma cov_45_0002 : covers (row_to_tm [t1RB;t1LC;t0LC;t0RB;t1LA;t1RD;t1RC;t1LB]).
+Proof.
+  apply (covers_iqh_at BBB4.Machines.NGHWStage.NGHW_03.tmq_h_00399);
+    [exact BBB4.Machines.NGHWStage.NGHW_03.cqh_h_00399 | intros q s; destruct q, s; reflexivity].
+Qed.
+
+(* 1RB1LC_1LC0RD_1LA0LB_1LD0RA *)
+Lemma cov_45_0003 : covers (row_to_tm [t1RB;t1LC;t1LC;t0RD;t1LA;t0LB;t1LD;t0RA]).
+Proof.
+  apply (covers_iqh_at BBB4.Machines.NGHWStage.NGHW_04.tmq_h_00400);
+    [exact BBB4.Machines.NGHWStage.NGHW_04.cqh_h_00400 | intros q s; destruct q, s; reflexivity].
+Qed.
+
 (* 1RB1LC_1LC1RD_0RB0LC_1RB0LA *)
-Lemma cov_45_0000 : covers (row_to_tm [t1RB;t1LC;t1LC;t1RD;t0RB;t0LC;t1RB;t0LA]).
+Lemma cov_45_0004 : covers (row_to_tm [t1RB;t1LC;t1LC;t1RD;t0RB;t0LC;t1RB;t0LA]).
 Proof.
   apply (covers_iqh_at BBB4.Machines.NGHWStage.NGHW_04.tmq_h_00401);
     [exact BBB4.Machines.NGHWStage.NGHW_04.cqh_h_00401 | intros q s; destruct q, s; reflexivity].
 Qed.
 
 (* 1RB1LC_1RC1LD_0LA0RD_1LD1LB *)
-Lemma cov_45_0001 : covers (row_to_tm [t1RB;t1LC;t1RC;t1LD;t0LA;t0RD;t1LD;t1LB]).
+Lemma cov_45_0005 : covers (row_to_tm [t1RB;t1LC;t1RC;t1LD;t0LA;t0RD;t1LD;t1LB]).
 Proof.
   apply (covers_iqh_at BBB4.Machines.NGHWStage.NGHW_04.tmq_h_00402);
     [exact BBB4.Machines.NGHWStage.NGHW_04.cqh_h_00402 | intros q s; destruct q, s; reflexivity].
 Qed.
 
 (* 1RB1LC_1RC1LD_0LB0RC_1LB0LA *)
-Lemma cov_45_0002 : covers (row_to_tm [t1RB;t1LC;t1RC;t1LD;t0LB;t0RC;t1LB;t0LA]).
+Lemma cov_45_0006 : covers (row_to_tm [t1RB;t1LC;t1RC;t1LD;t0LB;t0RC;t1LB;t0LA]).
 Proof.
   apply (covers_iqh_at BBB4.Machines.NGHWStage.NGHW_04.tmq_h_00403);
     [exact BBB4.Machines.NGHWStage.NGHW_04.cqh_h_00403 | intros q s; destruct q, s; reflexivity].
 Qed.
 
 (* 1RB1LC_1RC1LD_0LB0RC_1LB0RA *)
-Lemma cov_45_0003 : covers (row_to_tm [t1RB;t1LC;t1RC;t1LD;t0LB;t0RC;t1LB;t0RA]).
+Lemma cov_45_0007 : covers (row_to_tm [t1RB;t1LC;t1RC;t1LD;t0LB;t0RC;t1LB;t0RA]).
 Proof.
   apply (covers_iqh_at BBB4.Machines.NGHWStage.NGHW_04.tmq_h_00404);
     [exact BBB4.Machines.NGHWStage.NGHW_04.cqh_h_00404 | intros q s; destruct q, s; reflexivity].
 Qed.
 
 (* 1RB1LC_1RC1LD_0LB0RC_1LB1RA *)
-Lemma cov_45_0004 : covers (row_to_tm [t1RB;t1LC;t1RC;t1LD;t0LB;t0RC;t1LB;t1RA]).
+Lemma cov_45_0008 : covers (row_to_tm [t1RB;t1LC;t1RC;t1LD;t0LB;t0RC;t1LB;t1RA]).
 Proof.
   apply (covers_iqh_at BBB4.Machines.NGHWStage.NGHW_04.tmq_h_00405);
     [exact BBB4.Machines.NGHWStage.NGHW_04.cqh_h_00405 | intros q s; destruct q, s; reflexivity].
 Qed.
 
 (* 1RB1LC_1RC1LD_0LD0RC_1LB0LA *)
-Lemma cov_45_0005 : covers (row_to_tm [t1RB;t1LC;t1RC;t1LD;t0LD;t0RC;t1LB;t0LA]).
+Lemma cov_45_0009 : covers (row_to_tm [t1RB;t1LC;t1RC;t1LD;t0LD;t0RC;t1LB;t0LA]).
 Proof.
   apply (covers_iqh_at BBB4.Machines.NGHWStage.NGHW_04.tmq_h_00406);
     [exact BBB4.Machines.NGHWStage.NGHW_04.cqh_h_00406 | intros q s; destruct q, s; reflexivity].
 Qed.
 
 (* 1RB1LC_1RC1LD_0LD0RC_1LB1LA *)
-Lemma cov_45_0006 : covers (row_to_tm [t1RB;t1LC;t1RC;t1LD;t0LD;t0RC;t1LB;t1LA]).
+Lemma cov_45_0010 : covers (row_to_tm [t1RB;t1LC;t1RC;t1LD;t0LD;t0RC;t1LB;t1LA]).
 Proof.
   apply (covers_iqh_at BBB4.Machines.NGHWStage.NGHW_04.tmq_h_00407);
     [exact BBB4.Machines.NGHWStage.NGHW_04.cqh_h_00407 | intros q s; destruct q, s; reflexivity].
 Qed.
 
 (* 1RB1LD_0LC0RD_---1LA_1LD1LA *)
-Lemma cov_45_0007 : covers (row_to_tm [t1RB;t1LD;t0LC;t0RD;tN;t1LA;t1LD;t1LA]).
+Lemma cov_45_0011 : covers (row_to_tm [t1RB;t1LD;t0LC;t0RD;tN;t1LA;t1LD;t1LA]).
 Proof.
   apply (covers_iqh_at BBB4.Machines.NGHWStage.NGHW_04.tmq_h_00408);
     [exact BBB4.Machines.NGHWStage.NGHW_04.cqh_h_00408 | intros q s; destruct q, s; reflexivity].
 Qed.
 
 (* 1RB1LD_0LC0RD_0LD1RC_1LD1LA *)
-Lemma cov_45_0008 : covers (row_to_tm [t1RB;t1LD;t0LC;t0RD;t0LD;t1RC;t1LD;t1LA]).
+Lemma cov_45_0012 : covers (row_to_tm [t1RB;t1LD;t0LC;t0RD;t0LD;t1RC;t1LD;t1LA]).
 Proof.
   apply (covers_iqh_at BBB4.Machines.NGHWStage.NGHW_04.tmq_h_00409);
     [exact BBB4.Machines.NGHWStage.NGHW_04.cqh_h_00409 | intros q s; destruct q, s; reflexivity].
 Qed.
 
 (* 1RB1LD_0LC0RD_0RA1LB_1LD1LA *)
-Lemma cov_45_0009 : covers (row_to_tm [t1RB;t1LD;t0LC;t0RD;t0RA;t1LB;t1LD;t1LA]).
+Lemma cov_45_0013 : covers (row_to_tm [t1RB;t1LD;t0LC;t0RD;t0RA;t1LB;t1LD;t1LA]).
 Proof.
   apply (covers_iqh_at BBB4.Machines.NGHWStage.NGHW_04.tmq_h_00410);
     [exact BBB4.Machines.NGHWStage.NGHW_04.cqh_h_00410 | intros q s; destruct q, s; reflexivity].
 Qed.
 
 (* 1RB1LD_0LC0RD_0RD1LC_1LD1LA *)
-Lemma cov_45_0010 : covers (row_to_tm [t1RB;t1LD;t0LC;t0RD;t0RD;t1LC;t1LD;t1LA]).
+Lemma cov_45_0014 : covers (row_to_tm [t1RB;t1LD;t0LC;t0RD;t0RD;t1LC;t1LD;t1LA]).
 Proof.
   apply (covers_iqh_at BBB4.Machines.NGHWStage.NGHW_04.tmq_h_00411);
     [exact BBB4.Machines.NGHWStage.NGHW_04.cqh_h_00411 | intros q s; destruct q, s; reflexivity].
 Qed.
 
 (* 1RB1LD_0LC0RD_0RD1RC_1LD1LA *)
-Lemma cov_45_0011 : covers (row_to_tm [t1RB;t1LD;t0LC;t0RD;t0RD;t1RC;t1LD;t1LA]).
+Lemma cov_45_0015 : covers (row_to_tm [t1RB;t1LD;t0LC;t0RD;t0RD;t1RC;t1LD;t1LA]).
 Proof.
   apply (covers_iqh_at BBB4.Machines.NGHWStage.NGHW_04.tmq_h_00412);
     [exact BBB4.Machines.NGHWStage.NGHW_04.cqh_h_00412 | intros q s; destruct q, s; reflexivity].
 Qed.
 
 (* 1RB1LD_0LC0RD_1LA0LB_1LD1LA *)
-Lemma cov_45_0012 : covers (row_to_tm [t1RB;t1LD;t0LC;t0RD;t1LA;t0LB;t1LD;t1LA]).
+Lemma cov_45_0016 : covers (row_to_tm [t1RB;t1LD;t0LC;t0RD;t1LA;t0LB;t1LD;t1LA]).
 Proof.
   apply (covers_iqh_at BBB4.Machines.NGHWStage.NGHW_04.tmq_h_00413);
     [exact BBB4.Machines.NGHWStage.NGHW_04.cqh_h_00413 | intros q s; destruct q, s; reflexivity].
 Qed.
 
 (* 1RB1LD_0LC0RD_1LA0LC_1LD1LA *)
-Lemma cov_45_0013 : covers (row_to_tm [t1RB;t1LD;t0LC;t0RD;t1LA;t0LC;t1LD;t1LA]).
+Lemma cov_45_0017 : covers (row_to_tm [t1RB;t1LD;t0LC;t0RD;t1LA;t0LC;t1LD;t1LA]).
 Proof.
   apply (covers_iqh_at BBB4.Machines.NGHWStage.NGHW_04.tmq_h_00414);
     [exact BBB4.Machines.NGHWStage.NGHW_04.cqh_h_00414 | intros q s; destruct q, s; reflexivity].
 Qed.
 
 (* 1RB1LD_0LC0RD_1LA0RB_1LD1LA *)
-Lemma cov_45_0014 : covers (row_to_tm [t1RB;t1LD;t0LC;t0RD;t1LA;t0RB;t1LD;t1LA]).
+Lemma cov_45_0018 : covers (row_to_tm [t1RB;t1LD;t0LC;t0RD;t1LA;t0RB;t1LD;t1LA]).
 Proof.
   apply (covers_iqh_at BBB4.Machines.NGHWStage.NGHW_04.tmq_h_00415);
     [exact BBB4.Machines.NGHWStage.NGHW_04.cqh_h_00415 | intros q s; destruct q, s; reflexivity].
 Qed.
 
 (* 1RB1LD_0LC0RD_1LA0RC_1LD1LA *)
-Lemma cov_45_0015 : covers (row_to_tm [t1RB;t1LD;t0LC;t0RD;t1LA;t0RC;t1LD;t1LA]).
+Lemma cov_45_0019 : covers (row_to_tm [t1RB;t1LD;t0LC;t0RD;t1LA;t0RC;t1LD;t1LA]).
 Proof.
   apply (covers_iqh_at BBB4.Machines.NGHWStage.NGHW_04.tmq_h_00416);
     [exact BBB4.Machines.NGHWStage.NGHW_04.cqh_h_00416 | intros q s; destruct q, s; reflexivity].
 Qed.
 
 (* 1RB1LD_0LC0RD_1LB1RC_1LD1LA *)
-Lemma cov_45_0016 : covers (row_to_tm [t1RB;t1LD;t0LC;t0RD;t1LB;t1RC;t1LD;t1LA]).
+Lemma cov_45_0020 : covers (row_to_tm [t1RB;t1LD;t0LC;t0RD;t1LB;t1RC;t1LD;t1LA]).
 Proof.
   apply (covers_iqh_at BBB4.Machines.NGHWStage.NGHW_04.tmq_h_00417);
     [exact BBB4.Machines.NGHWStage.NGHW_04.cqh_h_00417 | intros q s; destruct q, s; reflexivity].
 Qed.
 
 (* 1RB1LD_0LC0RD_1RB1LC_1LD1LA *)
-Lemma cov_45_0017 : covers (row_to_tm [t1RB;t1LD;t0LC;t0RD;t1RB;t1LC;t1LD;t1LA]).
+Lemma cov_45_0021 : covers (row_to_tm [t1RB;t1LD;t0LC;t0RD;t1RB;t1LC;t1LD;t1LA]).
 Proof.
   apply (covers_iqh_at BBB4.Machines.NGHWStage.NGHW_04.tmq_h_00418);
     [exact BBB4.Machines.NGHWStage.NGHW_04.cqh_h_00418 | intros q s; destruct q, s; reflexivity].
 Qed.
 
 (* 1RB1LD_0LC0RD_1RD1LB_1LD1LA *)
-Lemma cov_45_0018 : covers (row_to_tm [t1RB;t1LD;t0LC;t0RD;t1RD;t1LB;t1LD;t1LA]).
+Lemma cov_45_0022 : covers (row_to_tm [t1RB;t1LD;t0LC;t0RD;t1RD;t1LB;t1LD;t1LA]).
 Proof.
   apply (covers_iqh_at BBB4.Machines.NGHWStage.NGHW_04.tmq_h_00419);
     [exact BBB4.Machines.NGHWStage.NGHW_04.cqh_h_00419 | intros q s; destruct q, s; reflexivity].
 Qed.
 
 (* 1RB1LD_0RC0RD_0LC1LA_1LD1LA *)
-Lemma cov_45_0019 : covers (row_to_tm [t1RB;t1LD;t0RC;t0RD;t0LC;t1LA;t1LD;t1LA]).
+Lemma cov_45_0023 : covers (row_to_tm [t1RB;t1LD;t0RC;t0RD;t0LC;t1LA;t1LD;t1LA]).
 Proof.
   apply (covers_iqh_at BBB4.Machines.NGHWStage.NGHW_04.tmq_h_00420);
     [exact BBB4.Machines.NGHWStage.NGHW_04.cqh_h_00420 | intros q s; destruct q, s; reflexivity].
 Qed.
 
 (* 1RB1LD_0RC0RD_1LB0LC_1LD1LA *)
-Lemma cov_45_0020 : covers (row_to_tm [t1RB;t1LD;t0RC;t0RD;t1LB;t0LC;t1LD;t1LA]).
+Lemma cov_45_0024 : covers (row_to_tm [t1RB;t1LD;t0RC;t0RD;t1LB;t0LC;t1LD;t1LA]).
 Proof.
   apply (covers_iqh_at BBB4.Machines.NGHWStage.NGHW_04.tmq_h_00421);
     [exact BBB4.Machines.NGHWStage.NGHW_04.cqh_h_00421 | intros q s; destruct q, s; reflexivity].
 Qed.
 
 (* 1RB1LD_0RC0RD_1LB1LD_1LD1LA *)
-Lemma cov_45_0021 : covers (row_to_tm [t1RB;t1LD;t0RC;t0RD;t1LB;t1LD;t1LD;t1LA]).
+Lemma cov_45_0025 : covers (row_to_tm [t1RB;t1LD;t0RC;t0RD;t1LB;t1LD;t1LD;t1LA]).
 Proof.
   apply (covers_iqh_at BBB4.Machines.NGHWStage.NGHW_04.tmq_h_00422);
     [exact BBB4.Machines.NGHWStage.NGHW_04.cqh_h_00422 | intros q s; destruct q, s; reflexivity].
 Qed.
 
 (* 1RB1LD_0RC0RD_1LB1RD_1LD1LA *)
-Lemma cov_45_0022 : covers (row_to_tm [t1RB;t1LD;t0RC;t0RD;t1LB;t1RD;t1LD;t1LA]).
+Lemma cov_45_0026 : covers (row_to_tm [t1RB;t1LD;t0RC;t0RD;t1LB;t1RD;t1LD;t1LA]).
 Proof.
   apply (covers_iqh_at BBB4.Machines.NGHWStage.NGHW_04.tmq_h_00423);
     [exact BBB4.Machines.NGHWStage.NGHW_04.cqh_h_00423 | intros q s; destruct q, s; reflexivity].
 Qed.
 
 (* 1RB1LD_0RC0RD_1LC0RB_1LD1LA *)
-Lemma cov_45_0023 : covers (row_to_tm [t1RB;t1LD;t0RC;t0RD;t1LC;t0RB;t1LD;t1LA]).
+Lemma cov_45_0027 : covers (row_to_tm [t1RB;t1LD;t0RC;t0RD;t1LC;t0RB;t1LD;t1LA]).
 Proof.
   apply (covers_iqh_at BBB4.Machines.NGHWStage.NGHW_04.tmq_h_00424);
     [exact BBB4.Machines.NGHWStage.NGHW_04.cqh_h_00424 | intros q s; destruct q, s; reflexivity].
 Qed.
 
 (* 1RB1LD_0RC0RD_1LC1LA_1LD1LA *)
-Lemma cov_45_0024 : covers (row_to_tm [t1RB;t1LD;t0RC;t0RD;t1LC;t1LA;t1LD;t1LA]).
+Lemma cov_45_0028 : covers (row_to_tm [t1RB;t1LD;t0RC;t0RD;t1LC;t1LA;t1LD;t1LA]).
 Proof.
   apply (covers_iqh_at BBB4.Machines.NGHWStage.NGHW_04.tmq_h_00425);
     [exact BBB4.Machines.NGHWStage.NGHW_04.cqh_h_00425 | intros q s; destruct q, s; reflexivity].
 Qed.
 
 (* 1RB1LD_0RC0RD_1LC1RA_1LD1LA *)
-Lemma cov_45_0025 : covers (row_to_tm [t1RB;t1LD;t0RC;t0RD;t1LC;t1RA;t1LD;t1LA]).
+Lemma cov_45_0029 : covers (row_to_tm [t1RB;t1LD;t0RC;t0RD;t1LC;t1RA;t1LD;t1LA]).
 Proof.
   apply (covers_iqh_at BBB4.Machines.NGHWStage.NGHW_04.tmq_h_00426);
     [exact BBB4.Machines.NGHWStage.NGHW_04.cqh_h_00426 | intros q s; destruct q, s; reflexivity].
 Qed.
 
 (* 1RB1LD_0RC0RD_1LD---_1LD1LA *)
-Lemma cov_45_0026 : covers (row_to_tm [t1RB;t1LD;t0RC;t0RD;t1LD;tN;t1LD;t1LA]).
+Lemma cov_45_0030 : covers (row_to_tm [t1RB;t1LD;t0RC;t0RD;t1LD;tN;t1LD;t1LA]).
 Proof.
   apply (covers_iqh_at BBB4.Machines.NGHWStage.NGHW_04.tmq_h_00427);
     [exact BBB4.Machines.NGHWStage.NGHW_04.cqh_h_00427 | intros q s; destruct q, s; reflexivity].
 Qed.
 
 (* 1RB1LD_0RC0RD_1RD---_1LD1LA *)
-Lemma cov_45_0027 : covers (row_to_tm [t1RB;t1LD;t0RC;t0RD;t1RD;tN;t1LD;t1LA]).
+Lemma cov_45_0031 : covers (row_to_tm [t1RB;t1LD;t0RC;t0RD;t1RD;tN;t1LD;t1LA]).
 Proof.
   apply (covers_iqh_at BBB4.Machines.NGHWStage.NGHW_04.tmq_h_00428);
     [exact BBB4.Machines.NGHWStage.NGHW_04.cqh_h_00428 | intros q s; destruct q, s; reflexivity].
 Qed.
 
 (* 1RB1LD_1LC0RA_1RD1LB_0LC0RD *)
-Lemma cov_45_0028 : covers (row_to_tm [t1RB;t1LD;t1LC;t0RA;t1RD;t1LB;t0LC;t0RD]).
+Lemma cov_45_0032 : covers (row_to_tm [t1RB;t1LD;t1LC;t0RA;t1RD;t1LB;t0LC;t0RD]).
 Proof.
   apply (covers_iqh_at BBB4.Machines.NGHWStage.NGHW_04.tmq_h_00429);
     [exact BBB4.Machines.NGHWStage.NGHW_04.cqh_h_00429 | intros q s; destruct q, s; reflexivity].
 Qed.
 
 (* 1RB1LD_1LC0RD_---0RD_1LD1LA *)
-Lemma cov_45_0029 : covers (row_to_tm [t1RB;t1LD;t1LC;t0RD;tN;t0RD;t1LD;t1LA]).
+Lemma cov_45_0033 : covers (row_to_tm [t1RB;t1LD;t1LC;t0RD;tN;t0RD;t1LD;t1LA]).
 Proof.
   apply (covers_iqh_at BBB4.Machines.NGHWStage.NGHW_04.tmq_h_00430);
     [exact BBB4.Machines.NGHWStage.NGHW_04.cqh_h_00430 | intros q s; destruct q, s; reflexivity].
 Qed.
 
 (* 1RB1LD_1LC0RD_---1RB_1LD1LA *)
-Lemma cov_45_0030 : covers (row_to_tm [t1RB;t1LD;t1LC;t0RD;tN;t1RB;t1LD;t1LA]).
+Lemma cov_45_0034 : covers (row_to_tm [t1RB;t1LD;t1LC;t0RD;tN;t1RB;t1LD;t1LA]).
 Proof.
   apply (covers_iqh_at BBB4.Machines.NGHWStage.NGHW_04.tmq_h_00431);
     [exact BBB4.Machines.NGHWStage.NGHW_04.cqh_h_00431 | intros q s; destruct q, s; reflexivity].
 Qed.
 
 (* 1RB1LD_1LC0RD_0LB1RC_1LD1LA *)
-Lemma cov_45_0031 : covers (row_to_tm [t1RB;t1LD;t1LC;t0RD;t0LB;t1RC;t1LD;t1LA]).
+Lemma cov_45_0035 : covers (row_to_tm [t1RB;t1LD;t1LC;t0RD;t0LB;t1RC;t1LD;t1LA]).
 Proof.
   apply (covers_iqh_at BBB4.Machines.NGHWStage.NGHW_04.tmq_h_00432);
     [exact BBB4.Machines.NGHWStage.NGHW_04.cqh_h_00432 | intros q s; destruct q, s; reflexivity].
 Qed.
 
 (* 1RB1LD_1LC0RD_0RA0LC_1LD1LA *)
-Lemma cov_45_0032 : covers (row_to_tm [t1RB;t1LD;t1LC;t0RD;t0RA;t0LC;t1LD;t1LA]).
+Lemma cov_45_0036 : covers (row_to_tm [t1RB;t1LD;t1LC;t0RD;t0RA;t0LC;t1LD;t1LA]).
 Proof.
   apply (covers_iqh_at BBB4.Machines.NGHWStage.NGHW_04.tmq_h_00433);
     [exact BBB4.Machines.NGHWStage.NGHW_04.cqh_h_00433 | intros q s; destruct q, s; reflexivity].
 Qed.
 
 (* 1RB1LD_1LC0RD_0RB0LC_1LD1LA *)
-Lemma cov_45_0033 : covers (row_to_tm [t1RB;t1LD;t1LC;t0RD;t0RB;t0LC;t1LD;t1LA]).
+Lemma cov_45_0037 : covers (row_to_tm [t1RB;t1LD;t1LC;t0RD;t0RB;t0LC;t1LD;t1LA]).
 Proof.
   apply (covers_iqh_at BBB4.Machines.NGHWStage.NGHW_04.tmq_h_00434);
     [exact BBB4.Machines.NGHWStage.NGHW_04.cqh_h_00434 | intros q s; destruct q, s; reflexivity].
 Qed.
 
 (* 1RB1LD_1LC0RD_0RB1LC_1LD1LA *)
-Lemma cov_45_0034 : covers (row_to_tm [t1RB;t1LD;t1LC;t0RD;t0RB;t1LC;t1LD;t1LA]).
+Lemma cov_45_0038 : covers (row_to_tm [t1RB;t1LD;t1LC;t0RD;t0RB;t1LC;t1LD;t1LA]).
 Proof.
   apply (covers_iqh_at BBB4.Machines.NGHWStage.NGHW_04.tmq_h_00435);
     [exact BBB4.Machines.NGHWStage.NGHW_04.cqh_h_00435 | intros q s; destruct q, s; reflexivity].
 Qed.
 
 (* 1RB1LD_1LC0RD_0RD1LB_1LD1LA *)
-Lemma cov_45_0035 : covers (row_to_tm [t1RB;t1LD;t1LC;t0RD;t0RD;t1LB;t1LD;t1LA]).
+Lemma cov_45_0039 : covers (row_to_tm [t1RB;t1LD;t1LC;t0RD;t0RD;t1LB;t1LD;t1LA]).
 Proof.
   apply (covers_iqh_at BBB4.Machines.NGHWStage.NGHW_04.tmq_h_00436);
     [exact BBB4.Machines.NGHWStage.NGHW_04.cqh_h_00436 | intros q s; destruct q, s; reflexivity].
 Qed.
 
 (* 1RB1LD_1LC0RD_1LA0RC_1LD1LA *)
-Lemma cov_45_0036 : covers (row_to_tm [t1RB;t1LD;t1LC;t0RD;t1LA;t0RC;t1LD;t1LA]).
+Lemma cov_45_0040 : covers (row_to_tm [t1RB;t1LD;t1LC;t0RD;t1LA;t0RC;t1LD;t1LA]).
 Proof.
   apply (covers_iqh_at BBB4.Machines.NGHWStage.NGHW_04.tmq_h_00437);
     [exact BBB4.Machines.NGHWStage.NGHW_04.cqh_h_00437 | intros q s; destruct q, s; reflexivity].
 Qed.
 
 (* 1RB1LD_1LC0RD_1LA1LC_1LD1LA *)
-Lemma cov_45_0037 : covers (row_to_tm [t1RB;t1LD;t1LC;t0RD;t1LA;t1LC;t1LD;t1LA]).
+Lemma cov_45_0041 : covers (row_to_tm [t1RB;t1LD;t1LC;t0RD;t1LA;t1LC;t1LD;t1LA]).
 Proof.
   apply (covers_iqh_at BBB4.Machines.NGHWStage.NGHW_04.tmq_h_00438);
     [exact BBB4.Machines.NGHWStage.NGHW_04.cqh_h_00438 | intros q s; destruct q, s; reflexivity].
 Qed.
 
 (* 1RB1LD_1LC0RD_1LA1RC_1LD1LA *)
-Lemma cov_45_0038 : covers (row_to_tm [t1RB;t1LD;t1LC;t0RD;t1LA;t1RC;t1LD;t1LA]).
+Lemma cov_45_0042 : covers (row_to_tm [t1RB;t1LD;t1LC;t0RD;t1LA;t1RC;t1LD;t1LA]).
 Proof.
   apply (covers_iqh_at BBB4.Machines.NGHWStage.NGHW_04.tmq_h_00439);
     [exact BBB4.Machines.NGHWStage.NGHW_04.cqh_h_00439 | intros q s; destruct q, s; reflexivity].
 Qed.
 
 (* 1RB1LD_1LC0RD_1RA1LC_1LD1LA *)
-Lemma cov_45_0039 : covers (row_to_tm [t1RB;t1LD;t1LC;t0RD;t1RA;t1LC;t1LD;t1LA]).
+Lemma cov_45_0043 : covers (row_to_tm [t1RB;t1LD;t1LC;t0RD;t1RA;t1LC;t1LD;t1LA]).
 Proof.
   apply (covers_iqh_at BBB4.Machines.NGHWStage.NGHW_04.tmq_h_00440);
     [exact BBB4.Machines.NGHWStage.NGHW_04.cqh_h_00440 | intros q s; destruct q, s; reflexivity].
 Qed.
 
 (* 1RB1LD_1LC0RD_1RB1LB_1LD1LA *)
-Lemma cov_45_0040 : covers (row_to_tm [t1RB;t1LD;t1LC;t0RD;t1RB;t1LB;t1LD;t1LA]).
+Lemma cov_45_0044 : covers (row_to_tm [t1RB;t1LD;t1LC;t0RD;t1RB;t1LB;t1LD;t1LA]).
 Proof.
   apply (covers_iqh_at BBB4.Machines.NGHWStage.NGHW_04.tmq_h_00441);
     [exact BBB4.Machines.NGHWStage.NGHW_04.cqh_h_00441 | intros q s; destruct q, s; reflexivity].
 Qed.
 
 (* 1RB1LD_1LC0RD_1RC1LB_1LD1LA *)
-Lemma cov_45_0041 : covers (row_to_tm [t1RB;t1LD;t1LC;t0RD;t1RC;t1LB;t1LD;t1LA]).
+Lemma cov_45_0045 : covers (row_to_tm [t1RB;t1LD;t1LC;t0RD;t1RC;t1LB;t1LD;t1LA]).
 Proof.
   apply (covers_iqh_at BBB4.Machines.NGHWStage.NGHW_04.tmq_h_00442);
     [exact BBB4.Machines.NGHWStage.NGHW_04.cqh_h_00442 | intros q s; destruct q, s; reflexivity].
 Qed.
 
 (* 1RB1LD_1LC0RD_1RD0LC_1LD1LA *)
-Lemma cov_45_0042 : covers (row_to_tm [t1RB;t1LD;t1LC;t0RD;t1RD;t0LC;t1LD;t1LA]).
+Lemma cov_45_0046 : covers (row_to_tm [t1RB;t1LD;t1LC;t0RD;t1RD;t0LC;t1LD;t1LA]).
 Proof.
   apply (covers_iqh_at BBB4.Machines.NGHWStage.NGHW_04.tmq_h_00443);
     [exact BBB4.Machines.NGHWStage.NGHW_04.cqh_h_00443 | intros q s; destruct q, s; reflexivity].
 Qed.
 
 (* 1RB1LD_1LC1LA_1RD1LB_0LC0RD *)
-Lemma cov_45_0043 : covers (row_to_tm [t1RB;t1LD;t1LC;t1LA;t1RD;t1LB;t0LC;t0RD]).
+Lemma cov_45_0047 : covers (row_to_tm [t1RB;t1LD;t1LC;t1LA;t1RD;t1LB;t0LC;t0RD]).
 Proof.
   apply (covers_iqh_at BBB4.Machines.NGHWStage.NGHW_04.tmq_h_00444);
     [exact BBB4.Machines.NGHWStage.NGHW_04.cqh_h_00444 | intros q s; destruct q, s; reflexivity].
 Qed.
 
 (* 1RB1LD_1LC1RA_0RB0LC_---0LB *)
-Lemma cov_45_0044 : covers (row_to_tm [t1RB;t1LD;t1LC;t1RA;t0RB;t0LC;tN;t0LB]).
+Lemma cov_45_0048 : covers (row_to_tm [t1RB;t1LD;t1LC;t1RA;t0RB;t0LC;tN;t0LB]).
 Proof.
   apply (covers_iqh_at BBB4.Machines.NGHWStage.NGHW_04.tmq_h_00445);
     [exact BBB4.Machines.NGHWStage.NGHW_04.cqh_h_00445 | intros q s; destruct q, s; reflexivity].
 Qed.
 
 (* 1RB1LD_1LC1RA_0RB0LC_---0RB *)
-Lemma cov_45_0045 : covers (row_to_tm [t1RB;t1LD;t1LC;t1RA;t0RB;t0LC;tN;t0RB]).
+Lemma cov_45_0049 : covers (row_to_tm [t1RB;t1LD;t1LC;t1RA;t0RB;t0LC;tN;t0RB]).
 Proof.
   apply (covers_iqh_at BBB4.Machines.NGHWStage.NGHW_04.tmq_h_00446);
     [exact BBB4.Machines.NGHWStage.NGHW_04.cqh_h_00446 | intros q s; destruct q, s; reflexivity].
 Qed.
 
 (* 1RB1LD_1LC1RA_0RB0LC_---0RC *)
-Lemma cov_45_0046 : covers (row_to_tm [t1RB;t1LD;t1LC;t1RA;t0RB;t0LC;tN;t0RC]).
+Lemma cov_45_0050 : covers (row_to_tm [t1RB;t1LD;t1LC;t1RA;t0RB;t0LC;tN;t0RC]).
 Proof.
   apply (covers_iqh_at BBB4.Machines.NGHWStage.NGHW_04.tmq_h_00447);
     [exact BBB4.Machines.NGHWStage.NGHW_04.cqh_h_00447 | intros q s; destruct q, s; reflexivity].
 Qed.
 
 (* 1RB1LD_1LC1RA_0RB0LC_---1RC *)
-Lemma cov_45_0047 : covers (row_to_tm [t1RB;t1LD;t1LC;t1RA;t0RB;t0LC;tN;t1RC]).
+Lemma cov_45_0051 : covers (row_to_tm [t1RB;t1LD;t1LC;t1RA;t0RB;t0LC;tN;t1RC]).
 Proof.
   apply (covers_iqh_at BBB4.Machines.NGHWStage.NGHW_04.tmq_h_00448);
     [exact BBB4.Machines.NGHWStage.NGHW_04.cqh_h_00448 | intros q s; destruct q, s; reflexivity].
 Qed.
 
 (* 1RB1LD_1LC1RA_0RB0LC_0LB0RA *)
-Lemma cov_45_0048 : covers (row_to_tm [t1RB;t1LD;t1LC;t1RA;t0RB;t0LC;t0LB;t0RA]).
+Lemma cov_45_0052 : covers (row_to_tm [t1RB;t1LD;t1LC;t1RA;t0RB;t0LC;t0LB;t0RA]).
 Proof.
   apply (covers_iqh_at BBB4.Machines.NGHWStage.NGHW_04.tmq_h_00449);
     [exact BBB4.Machines.NGHWStage.NGHW_04.cqh_h_00449 | intros q s; destruct q, s; reflexivity].
 Qed.
 
 (* 1RB1LD_1LC1RA_0RB0LC_0LB0RD *)
-Lemma cov_45_0049 : covers (row_to_tm [t1RB;t1LD;t1LC;t1RA;t0RB;t0LC;t0LB;t0RD]).
+Lemma cov_45_0053 : covers (row_to_tm [t1RB;t1LD;t1LC;t1RA;t0RB;t0LC;t0LB;t0RD]).
 Proof.
   apply (covers_iqh_at BBB4.Machines.NGHWStage.NGHW_04.tmq_h_00450);
     [exact BBB4.Machines.NGHWStage.NGHW_04.cqh_h_00450 | intros q s; destruct q, s; reflexivity].
 Qed.
 
 (* 1RB1LD_1LC1RA_0RB0LC_0LC0LD *)
-Lemma cov_45_0050 : covers (row_to_tm [t1RB;t1LD;t1LC;t1RA;t0RB;t0LC;t0LC;t0LD]).
+Lemma cov_45_0054 : covers (row_to_tm [t1RB;t1LD;t1LC;t1RA;t0RB;t0LC;t0LC;t0LD]).
 Proof.
   apply (covers_iqh_at BBB4.Machines.NGHWStage.NGHW_04.tmq_h_00451);
     [exact BBB4.Machines.NGHWStage.NGHW_04.cqh_h_00451 | intros q s; destruct q, s; reflexivity].
 Qed.
 
 (* 1RB1LD_1LC1RA_0RB0LC_0LC0RD *)
-Lemma cov_45_0051 : covers (row_to_tm [t1RB;t1LD;t1LC;t1RA;t0RB;t0LC;t0LC;t0RD]).
+Lemma cov_45_0055 : covers (row_to_tm [t1RB;t1LD;t1LC;t1RA;t0RB;t0LC;t0LC;t0RD]).
 Proof.
   apply (covers_iqh_at BBB4.Machines.NGHWStage.NGHW_04.tmq_h_00452);
     [exact BBB4.Machines.NGHWStage.NGHW_04.cqh_h_00452 | intros q s; destruct q, s; reflexivity].
 Qed.
 
 (* 1RB1LD_1LC1RA_0RB0LC_0LC1RD *)
-Lemma cov_45_0052 : covers (row_to_tm [t1RB;t1LD;t1LC;t1RA;t0RB;t0LC;t0LC;t1RD]).
+Lemma cov_45_0056 : covers (row_to_tm [t1RB;t1LD;t1LC;t1RA;t0RB;t0LC;t0LC;t1RD]).
 Proof.
   apply (covers_iqh_at BBB4.Machines.NGHWStage.NGHW_04.tmq_h_00453);
     [exact BBB4.Machines.NGHWStage.NGHW_04.cqh_h_00453 | intros q s; destruct q, s; reflexivity].
 Qed.
 
 (* 1RB1LD_1LC1RA_0RB0LC_0RB0RA *)
-Lemma cov_45_0053 : covers (row_to_tm [t1RB;t1LD;t1LC;t1RA;t0RB;t0LC;t0RB;t0RA]).
+Lemma cov_45_0057 : covers (row_to_tm [t1RB;t1LD;t1LC;t1RA;t0RB;t0LC;t0RB;t0RA]).
 Proof.
   apply (covers_iqh_at BBB4.Machines.NGHWStage.NGHW_04.tmq_h_00454);
     [exact BBB4.Machines.NGHWStage.NGHW_04.cqh_h_00454 | intros q s; destruct q, s; reflexivity].
 Qed.
 
 (* 1RB1LD_1LC1RA_0RB0LC_0RB0RD *)
-Lemma cov_45_0054 : covers (row_to_tm [t1RB;t1LD;t1LC;t1RA;t0RB;t0LC;t0RB;t0RD]).
+Lemma cov_45_0058 : covers (row_to_tm [t1RB;t1LD;t1LC;t1RA;t0RB;t0LC;t0RB;t0RD]).
 Proof.
   apply (covers_iqh_at BBB4.Machines.NGHWStage.NGHW_04.tmq_h_00455);
     [exact BBB4.Machines.NGHWStage.NGHW_04.cqh_h_00455 | intros q s; destruct q, s; reflexivity].
 Qed.
 
 (* 1RB1LD_1LC1RA_0RB0LC_0RB1RD *)
-Lemma cov_45_0055 : covers (row_to_tm [t1RB;t1LD;t1LC;t1RA;t0RB;t0LC;t0RB;t1RD]).
+Lemma cov_45_0059 : covers (row_to_tm [t1RB;t1LD;t1LC;t1RA;t0RB;t0LC;t0RB;t1RD]).
 Proof.
   apply (covers_iqh_at BBB4.Machines.NGHWStage.NGHW_04.tmq_h_00456);
     [exact BBB4.Machines.NGHWStage.NGHW_04.cqh_h_00456 | intros q s; destruct q, s; reflexivity].
 Qed.
 
 (* 1RB1LD_1LC1RA_0RB0LC_0RC0LD *)
-Lemma cov_45_0056 : covers (row_to_tm [t1RB;t1LD;t1LC;t1RA;t0RB;t0LC;t0RC;t0LD]).
+Lemma cov_45_0060 : covers (row_to_tm [t1RB;t1LD;t1LC;t1RA;t0RB;t0LC;t0RC;t0LD]).
 Proof.
   apply (covers_iqh_at BBB4.Machines.NGHWStage.NGHW_04.tmq_h_00457);
     [exact BBB4.Machines.NGHWStage.NGHW_04.cqh_h_00457 | intros q s; destruct q, s; reflexivity].
 Qed.
 
 (* 1RB1LD_1LC1RA_0RB0LC_0RC0RA *)
-Lemma cov_45_0057 : covers (row_to_tm [t1RB;t1LD;t1LC;t1RA;t0RB;t0LC;t0RC;t0RA]).
+Lemma cov_45_0061 : covers (row_to_tm [t1RB;t1LD;t1LC;t1RA;t0RB;t0LC;t0RC;t0RA]).
 Proof.
   apply (covers_iqh_at BBB4.Machines.NGHWStage.NGHW_04.tmq_h_00458);
     [exact BBB4.Machines.NGHWStage.NGHW_04.cqh_h_00458 | intros q s; destruct q, s; reflexivity].
 Qed.
 
 (* 1RB1LD_1LC1RA_0RB0LC_0RC0RD *)
-Lemma cov_45_0058 : covers (row_to_tm [t1RB;t1LD;t1LC;t1RA;t0RB;t0LC;t0RC;t0RD]).
+Lemma cov_45_0062 : covers (row_to_tm [t1RB;t1LD;t1LC;t1RA;t0RB;t0LC;t0RC;t0RD]).
 Proof.
   apply (covers_iqh_at BBB4.Machines.NGHWStage.NGHW_04.tmq_h_00459);
     [exact BBB4.Machines.NGHWStage.NGHW_04.cqh_h_00459 | intros q s; destruct q, s; reflexivity].
 Qed.
 
 (* 1RB1LD_1LC1RA_0RB0LC_0RC1RD *)
-Lemma cov_45_0059 : covers (row_to_tm [t1RB;t1LD;t1LC;t1RA;t0RB;t0LC;t0RC;t1RD]).
+Lemma cov_45_0063 : covers (row_to_tm [t1RB;t1LD;t1LC;t1RA;t0RB;t0LC;t0RC;t1RD]).
 Proof.
   apply (covers_iqh_at BBB4.Machines.NGHWStage.NGHW_04.tmq_h_00460);
     [exact BBB4.Machines.NGHWStage.NGHW_04.cqh_h_00460 | intros q s; destruct q, s; reflexivity].
 Qed.
 
 (* 1RB1LD_1LC1RA_0RB0LC_1LC0LD *)
-Lemma cov_45_0060 : covers (row_to_tm [t1RB;t1LD;t1LC;t1RA;t0RB;t0LC;t1LC;t0LD]).
+Lemma cov_45_0064 : covers (row_to_tm [t1RB;t1LD;t1LC;t1RA;t0RB;t0LC;t1LC;t0LD]).
 Proof.
   apply (covers_iqh_at BBB4.Machines.NGHWStage.NGHW_04.tmq_h_00461);
     [exact BBB4.Machines.NGHWStage.NGHW_04.cqh_h_00461 | intros q s; destruct q, s; reflexivity].
 Qed.
 
 (* 1RB1LD_1LC1RA_0RB0LC_1LC0RD *)
-Lemma cov_45_0061 : covers (row_to_tm [t1RB;t1LD;t1LC;t1RA;t0RB;t0LC;t1LC;t0RD]).
+Lemma cov_45_0065 : covers (row_to_tm [t1RB;t1LD;t1LC;t1RA;t0RB;t0LC;t1LC;t0RD]).
 Proof.
   apply (covers_iqh_at BBB4.Machines.NGHWStage.NGHW_04.tmq_h_00462);
     [exact BBB4.Machines.NGHWStage.NGHW_04.cqh_h_00462 | intros q s; destruct q, s; reflexivity].
 Qed.
 
 (* 1RB1LD_1LC1RA_0RB0LC_1LC1RD *)
-Lemma cov_45_0062 : covers (row_to_tm [t1RB;t1LD;t1LC;t1RA;t0RB;t0LC;t1LC;t1RD]).
+Lemma cov_45_0066 : covers (row_to_tm [t1RB;t1LD;t1LC;t1RA;t0RB;t0LC;t1LC;t1RD]).
 Proof.
   apply (covers_iqh_at BBB4.Machines.NGHWStage.NGHW_04.tmq_h_00463);
     [exact BBB4.Machines.NGHWStage.NGHW_04.cqh_h_00463 | intros q s; destruct q, s; reflexivity].
 Qed.
 
 (* 1RB1LD_1LC1RA_0RB0LC_1RA0LD *)
-Lemma cov_45_0063 : covers (row_to_tm [t1RB;t1LD;t1LC;t1RA;t0RB;t0LC;t1RA;t0LD]).
+Lemma cov_45_0067 : covers (row_to_tm [t1RB;t1LD;t1LC;t1RA;t0RB;t0LC;t1RA;t0LD]).
 Proof.
   apply (covers_iqh_at BBB4.Machines.NGHWStage.NGHW_04.tmq_h_00464);
     [exact BBB4.Machines.NGHWStage.NGHW_04.cqh_h_00464 | intros q s; destruct q, s; reflexivity].
 Qed.
 
 (* 1RB1LD_1LC1RA_0RB0LC_1RA0RD *)
-Lemma cov_45_0064 : covers (row_to_tm [t1RB;t1LD;t1LC;t1RA;t0RB;t0LC;t1RA;t0RD]).
+Lemma cov_45_0068 : covers (row_to_tm [t1RB;t1LD;t1LC;t1RA;t0RB;t0LC;t1RA;t0RD]).
 Proof.
   apply (covers_iqh_at BBB4.Machines.NGHWStage.NGHW_04.tmq_h_00465);
     [exact BBB4.Machines.NGHWStage.NGHW_04.cqh_h_00465 | intros q s; destruct q, s; reflexivity].
 Qed.
 
 (* 1RB1LD_1LC1RA_0RB0LC_1RA1RD *)
-Lemma cov_45_0065 : covers (row_to_tm [t1RB;t1LD;t1LC;t1RA;t0RB;t0LC;t1RA;t1RD]).
+Lemma cov_45_0069 : covers (row_to_tm [t1RB;t1LD;t1LC;t1RA;t0RB;t0LC;t1RA;t1RD]).
 Proof.
   apply (covers_iqh_at BBB4.Machines.NGHWStage.NGHW_04.tmq_h_00466);
     [exact BBB4.Machines.NGHWStage.NGHW_04.cqh_h_00466 | intros q s; destruct q, s; reflexivity].
 Qed.
 
 (* 1RB1LD_1LC1RA_0RB0LC_1RC0LD *)
-Lemma cov_45_0066 : covers (row_to_tm [t1RB;t1LD;t1LC;t1RA;t0RB;t0LC;t1RC;t0LD]).
+Lemma cov_45_0070 : covers (row_to_tm [t1RB;t1LD;t1LC;t1RA;t0RB;t0LC;t1RC;t0LD]).
 Proof.
   apply (covers_iqh_at BBB4.Machines.NGHWStage.NGHW_04.tmq_h_00467);
     [exact BBB4.Machines.NGHWStage.NGHW_04.cqh_h_00467 | intros q s; destruct q, s; reflexivity].
 Qed.
 
 (* 1RB1LD_1LC1RA_0RB0LC_1RC0RA *)
-Lemma cov_45_0067 : covers (row_to_tm [t1RB;t1LD;t1LC;t1RA;t0RB;t0LC;t1RC;t0RA]).
+Lemma cov_45_0071 : covers (row_to_tm [t1RB;t1LD;t1LC;t1RA;t0RB;t0LC;t1RC;t0RA]).
 Proof.
   apply (covers_iqh_at BBB4.Machines.NGHWStage.NGHW_04.tmq_h_00468);
     [exact BBB4.Machines.NGHWStage.NGHW_04.cqh_h_00468 | intros q s; destruct q, s; reflexivity].
 Qed.
 
 (* 1RB1LD_1LC1RA_0RB0LC_1RC0RD *)
-Lemma cov_45_0068 : covers (row_to_tm [t1RB;t1LD;t1LC;t1RA;t0RB;t0LC;t1RC;t0RD]).
+Lemma cov_45_0072 : covers (row_to_tm [t1RB;t1LD;t1LC;t1RA;t0RB;t0LC;t1RC;t0RD]).
 Proof.
   apply (covers_iqh_at BBB4.Machines.NGHWStage.NGHW_04.tmq_h_00469);
     [exact BBB4.Machines.NGHWStage.NGHW_04.cqh_h_00469 | intros q s; destruct q, s; reflexivity].
 Qed.
 
 (* 1RB1LD_1LC1RA_0RB0LC_1RC1LD *)
-Lemma cov_45_0069 : covers (row_to_tm [t1RB;t1LD;t1LC;t1RA;t0RB;t0LC;t1RC;t1LD]).
+Lemma cov_45_0073 : covers (row_to_tm [t1RB;t1LD;t1LC;t1RA;t0RB;t0LC;t1RC;t1LD]).
 Proof.
   apply (covers_iqh_at BBB4.Machines.NGHWStage.NGHW_04.tmq_h_00470);
     [exact BBB4.Machines.NGHWStage.NGHW_04.cqh_h_00470 | intros q s; destruct q, s; reflexivity].
 Qed.
 
 (* 1RB1LD_1LC1RA_0RB0LC_1RC1RD *)
-Lemma cov_45_0070 : covers (row_to_tm [t1RB;t1LD;t1LC;t1RA;t0RB;t0LC;t1RC;t1RD]).
+Lemma cov_45_0074 : covers (row_to_tm [t1RB;t1LD;t1LC;t1RA;t0RB;t0LC;t1RC;t1RD]).
 Proof.
   apply (covers_iqh_at BBB4.Machines.NGHWStage.NGHW_04.tmq_h_00471);
     [exact BBB4.Machines.NGHWStage.NGHW_04.cqh_h_00471 | intros q s; destruct q, s; reflexivity].
 Qed.
 
 (* 1RB1LD_1LC1RA_1RD1LB_0LC0RD *)
-Lemma cov_45_0071 : covers (row_to_tm [t1RB;t1LD;t1LC;t1RA;t1RD;t1LB;t0LC;t0RD]).
+Lemma cov_45_0075 : covers (row_to_tm [t1RB;t1LD;t1LC;t1RA;t1RD;t1LB;t0LC;t0RD]).
 Proof.
   apply (covers_iqh_at BBB4.Machines.NGHWStage.NGHW_04.tmq_h_00472);
     [exact BBB4.Machines.NGHWStage.NGHW_04.cqh_h_00472 | intros q s; destruct q, s; reflexivity].
 Qed.
 
 (* 1RB1LD_1RC0LA_1LD1RB_0RB0LD *)
-Lemma cov_45_0072 : covers (row_to_tm [t1RB;t1LD;t1RC;t0LA;t1LD;t1RB;t0RB;t0LD]).
+Lemma cov_45_0076 : covers (row_to_tm [t1RB;t1LD;t1RC;t0LA;t1LD;t1RB;t0RB;t0LD]).
 Proof.
   apply (covers_iqh_at BBB4.Machines.NGHWStage.NGHW_04.tmq_h_00473);
     [exact BBB4.Machines.NGHWStage.NGHW_04.cqh_h_00473 | intros q s; destruct q, s; reflexivity].
 Qed.
 
 (* 1RB1LD_1RC0RD_0LB---_1LD1LA *)
-Lemma cov_45_0073 : covers (row_to_tm [t1RB;t1LD;t1RC;t0RD;t0LB;tN;t1LD;t1LA]).
+Lemma cov_45_0077 : covers (row_to_tm [t1RB;t1LD;t1RC;t0RD;t0LB;tN;t1LD;t1LA]).
 Proof.
   apply (covers_iqh_at BBB4.Machines.NGHWStage.NGHW_04.tmq_h_00474);
     [exact BBB4.Machines.NGHWStage.NGHW_04.cqh_h_00474 | intros q s; destruct q, s; reflexivity].
 Qed.
 
 (* 1RB1LD_1RC0RD_0LC0LD_1LD1LA *)
-Lemma cov_45_0074 : covers (row_to_tm [t1RB;t1LD;t1RC;t0RD;t0LC;t0LD;t1LD;t1LA]).
+Lemma cov_45_0078 : covers (row_to_tm [t1RB;t1LD;t1RC;t0RD;t0LC;t0LD;t1LD;t1LA]).
 Proof.
   apply (covers_iqh_at BBB4.Machines.NGHWStage.NGHW_04.tmq_h_00475);
     [exact BBB4.Machines.NGHWStage.NGHW_04.cqh_h_00475 | intros q s; destruct q, s; reflexivity].
 Qed.
 
 (* 1RB1LD_1RC0RD_0LC0RD_1LD1LA *)
-Lemma cov_45_0075 : covers (row_to_tm [t1RB;t1LD;t1RC;t0RD;t0LC;t0RD;t1LD;t1LA]).
+Lemma cov_45_0079 : covers (row_to_tm [t1RB;t1LD;t1RC;t0RD;t0LC;t0RD;t1LD;t1LA]).
 Proof.
   apply (covers_iqh_at BBB4.Machines.NGHWStage.NGHW_04.tmq_h_00476);
     [exact BBB4.Machines.NGHWStage.NGHW_04.cqh_h_00476 | intros q s; destruct q, s; reflexivity].
 Qed.
 
 (* 1RB1LD_1RC0RD_0LC1LB_1LD1LA *)
-Lemma cov_45_0076 : covers (row_to_tm [t1RB;t1LD;t1RC;t0RD;t0LC;t1LB;t1LD;t1LA]).
+Lemma cov_45_0080 : covers (row_to_tm [t1RB;t1LD;t1RC;t0RD;t0LC;t1LB;t1LD;t1LA]).
 Proof.
   apply (covers_iqh_at BBB4.Machines.NGHWStage.NGHW_04.tmq_h_00477);
     [exact BBB4.Machines.NGHWStage.NGHW_04.cqh_h_00477 | intros q s; destruct q, s; reflexivity].
 Qed.
 
 (* 1RB1LD_1RC0RD_1LA---_1LD1LA *)
-Lemma cov_45_0077 : covers (row_to_tm [t1RB;t1LD;t1RC;t0RD;t1LA;tN;t1LD;t1LA]).
+Lemma cov_45_0081 : covers (row_to_tm [t1RB;t1LD;t1RC;t0RD;t1LA;tN;t1LD;t1LA]).
 Proof.
   apply (covers_iqh_at BBB4.Machines.NGHWStage.NGHW_04.tmq_h_00478);
     [exact BBB4.Machines.NGHWStage.NGHW_04.cqh_h_00478 | intros q s; destruct q, s; reflexivity].
 Qed.
 
 (* 1RB1LD_1RC0RD_1LC0RA_1LD1LA *)
-Lemma cov_45_0078 : covers (row_to_tm [t1RB;t1LD;t1RC;t0RD;t1LC;t0RA;t1LD;t1LA]).
+Lemma cov_45_0082 : covers (row_to_tm [t1RB;t1LD;t1RC;t0RD;t1LC;t0RA;t1LD;t1LA]).
 Proof.
   apply (covers_iqh_at BBB4.Machines.NGHWStage.NGHW_04.tmq_h_00479);
     [exact BBB4.Machines.NGHWStage.NGHW_04.cqh_h_00479 | intros q s; destruct q, s; reflexivity].
 Qed.
 
 (* 1RB1LD_1RC0RD_1LC1LD_1LD1LA *)
-Lemma cov_45_0079 : covers (row_to_tm [t1RB;t1LD;t1RC;t0RD;t1LC;t1LD;t1LD;t1LA]).
+Lemma cov_45_0083 : covers (row_to_tm [t1RB;t1LD;t1RC;t0RD;t1LC;t1LD;t1LD;t1LA]).
 Proof.
   apply (covers_iqh_at BBB4.Machines.NGHWStage.NGHW_04.tmq_h_00480);
     [exact BBB4.Machines.NGHWStage.NGHW_04.cqh_h_00480 | intros q s; destruct q, s; reflexivity].
 Qed.
 
 (* 1RB1LD_1RC0RD_1LC1RD_1LD1LA *)
-Lemma cov_45_0080 : covers (row_to_tm [t1RB;t1LD;t1RC;t0RD;t1LC;t1RD;t1LD;t1LA]).
+Lemma cov_45_0084 : covers (row_to_tm [t1RB;t1LD;t1RC;t0RD;t1LC;t1RD;t1LD;t1LA]).
 Proof.
   apply (covers_iqh_at BBB4.Machines.NGHWStage.NGHW_04.tmq_h_00481);
     [exact BBB4.Machines.NGHWStage.NGHW_04.cqh_h_00481 | intros q s; destruct q, s; reflexivity].
 Qed.
 
 (* 1RB1LD_1RC1LD_0LB0RC_1LB0LA *)
-Lemma cov_45_0081 : covers (row_to_tm [t1RB;t1LD;t1RC;t1LD;t0LB;t0RC;t1LB;t0LA]).
+Lemma cov_45_0085 : covers (row_to_tm [t1RB;t1LD;t1RC;t1LD;t0LB;t0RC;t1LB;t0LA]).
 Proof.
   apply (covers_iqh_at BBB4.Machines.NGHWStage.NGHW_04.tmq_h_00482);
     [exact BBB4.Machines.NGHWStage.NGHW_04.cqh_h_00482 | intros q s; destruct q, s; reflexivity].
 Qed.
 
 (* 1RB1LD_1RC1LD_0LB0RC_1LB0RA *)
-Lemma cov_45_0082 : covers (row_to_tm [t1RB;t1LD;t1RC;t1LD;t0LB;t0RC;t1LB;t0RA]).
+Lemma cov_45_0086 : covers (row_to_tm [t1RB;t1LD;t1RC;t1LD;t0LB;t0RC;t1LB;t0RA]).
 Proof.
   apply (covers_iqh_at BBB4.Machines.NGHWStage.NGHW_04.tmq_h_00483);
     [exact BBB4.Machines.NGHWStage.NGHW_04.cqh_h_00483 | intros q s; destruct q, s; reflexivity].
 Qed.
 
 (* 1RB1LD_1RC1LD_0LD0RC_1LB1LA *)
-Lemma cov_45_0083 : covers (row_to_tm [t1RB;t1LD;t1RC;t1LD;t0LD;t0RC;t1LB;t1LA]).
+Lemma cov_45_0087 : covers (row_to_tm [t1RB;t1LD;t1RC;t1LD;t0LD;t0RC;t1LB;t1LA]).
 Proof.
   apply (covers_iqh_at BBB4.Machines.NGHWStage.NGHW_04.tmq_h_00484);
     [exact BBB4.Machines.NGHWStage.NGHW_04.cqh_h_00484 | intros q s; destruct q, s; reflexivity].
 Qed.
 
 (* 1RB1LD_1RC1LD_1LA0RD_1LD1LB *)
-Lemma cov_45_0084 : covers (row_to_tm [t1RB;t1LD;t1RC;t1LD;t1LA;t0RD;t1LD;t1LB]).
+Lemma cov_45_0088 : covers (row_to_tm [t1RB;t1LD;t1RC;t1LD;t1LA;t0RD;t1LD;t1LB]).
 Proof.
   apply (covers_iqh_at BBB4.Machines.NGHWStage.NGHW_04.tmq_h_00485);
     [exact BBB4.Machines.NGHWStage.NGHW_04.cqh_h_00485 | intros q s; destruct q, s; reflexivity].
 Qed.
 
 (* 1RB1RA_1LC1RD_0RB0LC_1RB0LA *)
-Lemma cov_45_0085 : covers (row_to_tm [t1RB;t1RA;t1LC;t1RD;t0RB;t0LC;t1RB;t0LA]).
+Lemma cov_45_0089 : covers (row_to_tm [t1RB;t1RA;t1LC;t1RD;t0RB;t0LC;t1RB;t0LA]).
 Proof.
   apply (covers_iqh_at BBB4.Machines.NGHWStage.NGHW_04.tmq_h_00486);
     [exact BBB4.Machines.NGHWStage.NGHW_04.cqh_h_00486 | intros q s; destruct q, s; reflexivity].
 Qed.
 
 (* 1RB1RA_1RC1LA_1LD1RB_0RB0LD *)
-Lemma cov_45_0086 : covers (row_to_tm [t1RB;t1RA;t1RC;t1LA;t1LD;t1RB;t0RB;t0LD]).
+Lemma cov_45_0090 : covers (row_to_tm [t1RB;t1RA;t1RC;t1LA;t1LD;t1RB;t0RB;t0LD]).
 Proof.
   apply (covers_iqh_at BBB4.Machines.NGHWStage.NGHW_04.tmq_h_00487);
     [exact BBB4.Machines.NGHWStage.NGHW_04.cqh_h_00487 | intros q s; destruct q, s; reflexivity].
 Qed.
 
 (* 1RB1RB_1LA0LC_1RC1RD_1LB1RC *)
-Lemma cov_45_0087 : covers (row_to_tm [t1RB;t1RB;t1LA;t0LC;t1RC;t1RD;t1LB;t1RC]).
+Lemma cov_45_0091 : covers (row_to_tm [t1RB;t1RB;t1LA;t0LC;t1RC;t1RD;t1LB;t1RC]).
 Proof.
   apply (covers_iqh_at BBB4.Machines.NGHWStage.NGHW_04.tmq_h_00488);
     [exact BBB4.Machines.NGHWStage.NGHW_04.cqh_h_00488 | intros q s; destruct q, s; reflexivity].
 Qed.
 
 (* 1RB1RB_1LA0RC_1LC1LD_1RB1LC *)
-Lemma cov_45_0088 : covers (row_to_tm [t1RB;t1RB;t1LA;t0RC;t1LC;t1LD;t1RB;t1LC]).
+Lemma cov_45_0092 : covers (row_to_tm [t1RB;t1RB;t1LA;t0RC;t1LC;t1LD;t1RB;t1LC]).
 Proof.
   apply (covers_iqh_at BBB4.Machines.NGHWStage.NGHW_04.tmq_h_00489);
     [exact BBB4.Machines.NGHWStage.NGHW_04.cqh_h_00489 | intros q s; destruct q, s; reflexivity].
 Qed.
 
 (* 1RB1RB_1RC0LA_1LD1RB_0RB0LD *)
-Lemma cov_45_0089 : covers (row_to_tm [t1RB;t1RB;t1RC;t0LA;t1LD;t1RB;t0RB;t0LD]).
+Lemma cov_45_0093 : covers (row_to_tm [t1RB;t1RB;t1RC;t0LA;t1LD;t1RB;t0RB;t0LD]).
 Proof.
   apply (covers_iqh_at BBB4.Machines.NGHWStage.NGHW_04.tmq_h_00490);
     [exact BBB4.Machines.NGHWStage.NGHW_04.cqh_h_00490 | intros q s; destruct q, s; reflexivity].
 Qed.
 
 (* 1RB1RC_0LA0LD_1LB1RD_1RD1RC *)
-Lemma cov_45_0090 : covers (row_to_tm [t1RB;t1RC;t0LA;t0LD;t1LB;t1RD;t1RD;t1RC]).
+Lemma cov_45_0094 : covers (row_to_tm [t1RB;t1RC;t0LA;t0LD;t1LB;t1RD;t1RD;t1RC]).
 Proof.
   apply (covers_iqh_at BBB4.Machines.NGHWStage.NGHW_04.tmq_h_00491);
     [exact BBB4.Machines.NGHWStage.NGHW_04.cqh_h_00491 | intros q s; destruct q, s; reflexivity].
 Qed.
 
 (* 1RB1RC_1LC1RD_0RB0LC_1RB0LA *)
-Lemma cov_45_0091 : covers (row_to_tm [t1RB;t1RC;t1LC;t1RD;t0RB;t0LC;t1RB;t0LA]).
+Lemma cov_45_0095 : covers (row_to_tm [t1RB;t1RC;t1LC;t1RD;t0RB;t0LC;t1RB;t0LA]).
 Proof.
   apply (covers_iqh_at BBB4.Machines.NGHWStage.NGHW_04.tmq_h_00492);
     [exact BBB4.Machines.NGHWStage.NGHW_04.cqh_h_00492 | intros q s; destruct q, s; reflexivity].
 Qed.
 
 (* 1RB1RC_1LC1RD_0RB0LC_1RB1LA *)
-Lemma cov_45_0092 : covers (row_to_tm [t1RB;t1RC;t1LC;t1RD;t0RB;t0LC;t1RB;t1LA]).
+Lemma cov_45_0096 : covers (row_to_tm [t1RB;t1RC;t1LC;t1RD;t0RB;t0LC;t1RB;t1LA]).
 Proof.
   apply (covers_iqh_at BBB4.Machines.NGHWStage.NGHW_04.tmq_h_00493);
     [exact BBB4.Machines.NGHWStage.NGHW_04.cqh_h_00493 | intros q s; destruct q, s; reflexivity].
 Qed.
 
 (* 1RB1RC_1RC1LD_0LB0RC_1LB0LA *)
-Lemma cov_45_0093 : covers (row_to_tm [t1RB;t1RC;t1RC;t1LD;t0LB;t0RC;t1LB;t0LA]).
+Lemma cov_45_0097 : covers (row_to_tm [t1RB;t1RC;t1RC;t1LD;t0LB;t0RC;t1LB;t0LA]).
 Proof.
   apply (covers_iqh_at BBB4.Machines.NGHWStage.NGHW_04.tmq_h_00494);
     [exact BBB4.Machines.NGHWStage.NGHW_04.cqh_h_00494 | intros q s; destruct q, s; reflexivity].
 Qed.
 
 (* 1RB1RC_1RC1LD_0LB0RC_1LB0RA *)
-Lemma cov_45_0094 : covers (row_to_tm [t1RB;t1RC;t1RC;t1LD;t0LB;t0RC;t1LB;t0RA]).
+Lemma cov_45_0098 : covers (row_to_tm [t1RB;t1RC;t1RC;t1LD;t0LB;t0RC;t1LB;t0RA]).
 Proof.
   apply (covers_iqh_at BBB4.Machines.NGHWStage.NGHW_04.tmq_h_00495);
     [exact BBB4.Machines.NGHWStage.NGHW_04.cqh_h_00495 | intros q s; destruct q, s; reflexivity].
 Qed.
 
 (* 1RB1RC_1RC1LD_0LD0RC_1LB1LA *)
-Lemma cov_45_0095 : covers (row_to_tm [t1RB;t1RC;t1RC;t1LD;t0LD;t0RC;t1LB;t1LA]).
+Lemma cov_45_0099 : covers (row_to_tm [t1RB;t1RC;t1RC;t1LD;t0LD;t0RC;t1LB;t1LA]).
 Proof.
   apply (covers_iqh_at BBB4.Machines.NGHWStage.NGHW_04.tmq_h_00496);
     [exact BBB4.Machines.NGHWStage.NGHW_04.cqh_h_00496 | intros q s; destruct q, s; reflexivity].
 Qed.
 
-(* 1RB1RD_1LC0RA_1RD1LB_0LC0RD *)
-Lemma cov_45_0096 : covers (row_to_tm [t1RB;t1RD;t1LC;t0RA;t1RD;t1LB;t0LC;t0RD]).
-Proof.
-  apply (covers_iqh_at BBB4.Machines.NGHWStage.NGHW_04.tmq_h_00497);
-    [exact BBB4.Machines.NGHWStage.NGHW_04.cqh_h_00497 | intros q s; destruct q, s; reflexivity].
-Qed.
-
-(* 1RB1RD_1LC1LA_1RD1LB_0LC0RD *)
-Lemma cov_45_0097 : covers (row_to_tm [t1RB;t1RD;t1LC;t1LA;t1RD;t1LB;t0LC;t0RD]).
-Proof.
-  apply (covers_iqh_at BBB4.Machines.NGHWStage.NGHW_04.tmq_h_00498);
-    [exact BBB4.Machines.NGHWStage.NGHW_04.cqh_h_00498 | intros q s; destruct q, s; reflexivity].
-Qed.
-
-(* 1RB1RD_1LC1RA_0RB0LC_0LC--- *)
-Lemma cov_45_0098 : covers (row_to_tm [t1RB;t1RD;t1LC;t1RA;t0RB;t0LC;t0LC;tN]).
-Proof.
-  apply (covers_iqh_at BBB4.Machines.NGHWStage.NGHW_04.tmq_h_00499);
-    [exact BBB4.Machines.NGHWStage.NGHW_04.cqh_h_00499 | intros q s; destruct q, s; reflexivity].
-Qed.
-
-(* 1RB1RD_1LC1RA_0RB0LC_0LD0LB *)
-Lemma cov_45_0099 : covers (row_to_tm [t1RB;t1RD;t1LC;t1RA;t0RB;t0LC;t0LD;t0LB]).
-Proof.
-  apply (covers_iqh_at BBB4.Machines.NGHWStage.NGHW_05.tmq_h_00500);
-    [exact BBB4.Machines.NGHWStage.NGHW_05.cqh_h_00500 | intros q s; destruct q, s; reflexivity].
-Qed.
-
 Definition cbrows_45 : list (list (option Trans)) := [
+  [t1RB;t1LC;t0LC;t0RB;t1LA;t1RD;t1RC;t0LB];
+  [t1RB;t1LC;t0LC;t0RB;t1LA;t1RD;t1RC;t0LD];
+  [t1RB;t1LC;t0LC;t0RB;t1LA;t1RD;t1RC;t1LB];
+  [t1RB;t1LC;t1LC;t0RD;t1LA;t0LB;t1LD;t0RA];
   [t1RB;t1LC;t1LC;t1RD;t0RB;t0LC;t1RB;t0LA];
   [t1RB;t1LC;t1RC;t1LD;t0LA;t0RD;t1LD;t1LB];
   [t1RB;t1LC;t1RC;t1LD;t0LB;t0RC;t1LB;t0LA];
@@ -804,11 +808,7 @@ Definition cbrows_45 : list (list (option Trans)) := [
   [t1RB;t1RC;t1LC;t1RD;t0RB;t0LC;t1RB;t1LA];
   [t1RB;t1RC;t1RC;t1LD;t0LB;t0RC;t1LB;t0LA];
   [t1RB;t1RC;t1RC;t1LD;t0LB;t0RC;t1LB;t0RA];
-  [t1RB;t1RC;t1RC;t1LD;t0LD;t0RC;t1LB;t1LA];
-  [t1RB;t1RD;t1LC;t0RA;t1RD;t1LB;t0LC;t0RD];
-  [t1RB;t1RD;t1LC;t1LA;t1RD;t1LB;t0LC;t0RD];
-  [t1RB;t1RD;t1LC;t1RA;t0RB;t0LC;t0LC;tN];
-  [t1RB;t1RD;t1LC;t1RA;t0RB;t0LC;t0LD;t0LB]
+  [t1RB;t1RC;t1RC;t1LD;t0LD;t0RC;t1LB;t1LA]
 ].
 
 Lemma cb_45_covers : Forall covers (map row_to_tm cbrows_45).
